Moving semantics to Traces.v and doing some POR in ContextReduction setting

ContextReduction.v
@@ -1,6 +1,8 @@
 (** * Semantics by Head reductions in context *)
 
 From Coq Require Import String Bool Datatypes Relations Program.Equality.
+From Coq Require Import Classes.RelationClasses.
+From Coq Require Import Logic.FunctionalExtensionality. (* for equality of substitutions *)
 
 From SymEx Require Import Expr.
 Import BasicExpr.
@@ -8,6 +10,7 @@ Import BasicExpr.
 From SymEx Require Import Parallel.
 
 From SymEx Require Import Traces.
+Import TraceSemantics.
 
 From SymEx Require Import Maps.
 Import BasicMaps.
@@ -30,19 +33,33 @@ Inductive is_context: (Stmt -> Stmt) -> Prop :=
     is_context C -> is_context (fun x => SPar s (C x))
 .
 
-Inductive context_red {X:Type} (head_red: relation (X * Stmt) ): (X * Stmt) -> (X * Stmt) -> Prop :=
+Inductive context_red {X:Type} (head_red: relation (X * Stmt)): (X * Stmt) -> (X * Stmt) -> Prop :=
 | ctx_red_intro: forall C t t' s s',
     head_red (t, s) (t', s') -> is_context C ->
     context_red head_red (t, C s) (t', C s')
 .
 
+(* properties of contexts *)
+Lemma context_comp: forall C C', is_context C -> is_context C' -> is_context (fun s => C (C' s)).
+Proof. intros. induction H; induction H0; constructor; assumption. Qed.
+
+Lemma under_C {X: Type} (r: relation (X * Stmt)): forall C s s' t t',
+    context_red r (t, s) (t', s') -> is_context C -> context_red r (t, C s) (t', C s').
+Proof.
+  intros. dependent destruction H. apply ctx_red_intro with (C := fun s => C (C0 s)).
+  - assumption.
+  - apply context_comp; assumption.
+Qed.
+
+Lemma context_injective: forall C s s',
+    is_context C -> C s = C s' -> s = s'.
+Proof.
+  intros. induction H;
+    try (inversion H0; apply IHis_context);
+    assumption.
+Qed.
+
 (** Symbolic Semantics *)
-Inductive trace_step__S : Type :=
-| Asgn__S (x:Var) (e:Aexpr)
-| Cond (b:Bexpr).
-
-Definition trace__S := trace trace_step__S.
-
 Inductive head_red__S: (trace__S * Stmt) -> (trace__S * Stmt) -> Prop :=
 | head_red_asgn__S: forall t x e,
     head_red__S (t, <{ x := e }>) (t :: Asgn__S x e, SSkip)
@@ -98,22 +115,6 @@ Qed.
 
 (** Concrete Semantics *)
 
-Definition Val : Type := nat.
-Definition trace__C := trace (Var * Val).
-
-Fixpoint acc_val (V0:Valuation) (t:trace__C) : Valuation :=
-  match t with
-  | [] => V0
-  | t :: (x, v) => let V := acc_val V0 t in
-                 (x !-> v ; V)
-  end.
-
-Definition Aeval_t (V0:Valuation) (t:trace__C) (e:Aexpr) : nat :=
-  Aeval (acc_val V0 t) e.
-
-Definition Beval_t (V0:Valuation) (t:trace__C) (e:Bexpr) : bool :=
-  Beval (acc_val V0 t) e.
-
 Inductive head_red__C (V0:Valuation): (trace__C * Stmt) -> (trace__C * Stmt) -> Prop :=
 | head_red_asgn__C: forall t x e,
     head_red__C V0 (t, <{ x := e }>) (t :: (x, Aeval_t V0 t e), SSkip)
@@ -132,27 +133,6 @@ Definition red__C (V0:Valuation) := context_red (head_red__C V0).
 Definition red_star__C (V0:Valuation) := clos_refl_trans_n1 _ (red__C V0).
 
 (** Properties *)
-Fixpoint acc_subst (s0:sub) (t:trace__S) : sub :=
-  match t with
-  | [] => s0
-  | t :: Asgn__S x e => let s := acc_subst s0 t in
-                     (x !-> Aapply s e ; s)
-  | t :: _ => acc_subst s0 t
-  end.
-
-Definition Aapply_t (t:trace__S) (e:Aexpr) : Aexpr :=
-  Aapply (acc_subst id_sub t) e.
-
-Definition Bapply_t (t:trace__S) (e:Bexpr) : Bexpr :=
-  Bapply (acc_subst id_sub t) e.
-
-Fixpoint pc (t:trace__S) : Bexpr :=
-  match t with
-  | [] => BTrue
-  | t :: Cond b => BAnd (Bapply_t t b) (pc t)
-  | t :: _ => pc t
-  end.
-
 Lemma pc_monotone_step : forall V0 s1 s2 t1 t2, red__S (t1, s1) (t2, s2) -> Beval V0 (pc t2) = true -> Beval V0 (pc t1) = true.
 Proof. intros. inversion H. inversion H4; subst;
          simpl in H0; try (apply andb_true_iff in H0; destruct H0); assumption.
@@ -207,9 +187,6 @@ Proof.
     + assumption.
 Qed.
 
-Definition is_abstraction (V0:Valuation) (t:trace__C) (t':trace__S) : Prop :=
-  Beval V0 (pc t') = true /\ Comp V0 (acc_subst id_sub t') = acc_val V0 t.
-
 Lemma completeness_step : forall s s' t0 t t0' V0,
     red__C V0 (t0, s) (t, s') ->
     is_abstraction V0 t0 t0' ->
@@ -253,9 +230,225 @@ Proof.
   - destruct y. edestruct IHclos_refl_trans_n1 as [t' [IHcomp [IHpc IHabs]]];
       try reflexivity; try assumption.
     destruct (completeness_step _ _ _ _ t' _ H) as [t_step [Hstep [Hpc Habs]]]; try assumption.
-    split. assumption. assumption.
+    split; assumption.
     eexists. splits.
     + econstructor. apply Hstep. apply IHcomp.
     + apply Hpc.
     + apply Habs.
+Qed.
+
+(** * Sympaths - Trying out some stuff from Sympaths paper*)
+(* No thread identifiers, idk how that complicates things yet*)
+
+Fixpoint contains__A (e:Aexpr) (x:Var) : Prop :=
+  match e with
+  | AConst _ => False
+  | AVar y => x = y
+  | <{e1 + e2}> => contains__A e1 x \/ contains__A e2 x
+  end.
+
+Fixpoint contains__B (e:Bexpr) (x:Var) : Prop :=
+  match e with
+  | BTrue => False
+  | BFalse => False
+  | <{ ~ b }> => contains__B b x
+  | <{ b1 && b2 }> => contains__B b1 x \/ contains__B b2 x
+  | <{ a1 <= a2 }> => contains__A a1 x \/ contains__A a2 x
+  end.
+
+Definition reads_var (s:trace_step__S) (x:Var) : Prop :=
+  match s with
+  | Asgn__S _ e => contains__A e x
+  | Cond b => contains__B b x
+  end.
+
+Definition writes_var (s:trace_step__S) (x:Var) : Prop :=
+  match s with
+  | Asgn__S y e => x = y
+  | Cond b => False
+  end.
+
+Definition interference_free: relation trace_step__S :=
+  fun s1 s2 =>
+    forall x,
+      ~ (reads_var s1 x /\ writes_var s2 x) /\
+      ~ (writes_var s1 x /\ reads_var s2 x) /\
+      ~ (writes_var s1 x /\ writes_var s2 x).
+
+Global Instance sym_interference_free : Symmetric interference_free.
+Proof.
+  unfold interference_free. intros s1 s2 H x. specialize (H x). splits.
+  - destruct H as [_ [contra _]]. intro. destruct H. apply contra. splits; assumption.
+  - destruct H as [contra [_ _]]. intro. destruct H. apply contra. splits; assumption.
+  - destruct H as [_ [_ contra]]. intro. destruct H. apply contra. splits; assumption.
+Qed.
+
+Lemma interference_free_different_var: forall x x' e e', interference_free (Asgn__S x e) (Asgn__S x' e') -> x <> x'.
+Proof.
+  intros. intro contra. subst.
+  specialize (H x'). destruct H as [_ [_ H2]].
+  simpl in H2. apply H2. split; reflexivity.
+Qed.
+
+Lemma interference_free_different_expr: forall x x' e x0, interference_free (Asgn__S x e) (Asgn__S x' (AVar x0)) -> x <> x0.
+Proof.
+  intros. intro contra. subst.
+  specialize (H x0). destruct H as [_ [H1 _]].
+  simpl in H1. apply H1. split; reflexivity.
+Qed.
+
+Lemma IF_add_monotone: forall x x' e e1 e2,
+    interference_free (Asgn__S x e) (Asgn__S x' <{e1 + e2}>) ->
+    interference_free (Asgn__S x e) (Asgn__S x' e1) /\ interference_free (Asgn__S x e) (Asgn__S x' e2).
+Proof.
+  intros. split.
+  - intro y. specialize (H y). splits.
+    + destruct H as [H _]. intro contra. destruct contra.
+      apply H. split.
+      * assumption.
+      * inversion H1. reflexivity.
+    + destruct H as [_ [H _]]. intro contra. destruct contra.
+      apply H. split.
+      * assumption.
+      * unfold reads_var in *. destruct e2;
+          simpl; left; assumption.
+    + destruct H as [_ [_ H]]. intro contra. destruct contra.
+      apply H. split.
+      * assumption.
+      * inversion H1. reflexivity.
+  - intro y. specialize (H y). splits.
+    + destruct H as [H _]. intro contra. destruct contra.
+      apply H. split.
+      * assumption.
+      * inversion H1. reflexivity.
+    + destruct H as [_ [H _]]. intro contra. destruct contra.
+      apply H. split.
+      * assumption.
+      * unfold reads_var in *. destruct e1;
+          simpl; right; assumption.
+    + destruct H as [_ [_ H]]. intro contra. destruct contra.
+      apply H. split.
+      * assumption.
+      * inversion H1. reflexivity.
+Qed.
+
+Lemma IF_apply: forall s x x' e e',
+    interference_free (Asgn__S x e) (Asgn__S x' e') ->
+    (Aapply s e') = (Aapply (x !-> Aapply s e; s) e').
+Proof.
+  induction e'; intro IF.
+  - reflexivity.
+  - symmetry. apply update_neq. eapply interference_free_different_expr. apply IF.
+  - destruct (IF_add_monotone _ _ _ _ _ IF). simpl. rewrite IHe'1, IHe'2.
+    reflexivity.
+    all: assumption.
+Qed.
+
+Lemma IF_simultaneous_subst: forall s x x' e e',
+    interference_free (Asgn__S x e) (Asgn__S x' e') ->
+    (x' !-> Aapply (x !-> Aapply s e; s) e'; x !-> Aapply s e; s) =
+    (x !-> Aapply (x' !-> Aapply s e'; s) e; x' !-> Aapply s e'; s).
+Proof.
+  intros. specialize (interference_free_different_var _ _ _ _ H). intro.
+  rewrite update_comm.
+  replace (Aapply (x !-> Aapply s e; s) e') with (Aapply s e').
+  replace (Aapply (x' !-> Aapply s e'; s) e) with (Aapply s e).
+  reflexivity.
+  eapply IF_apply. symmetry in H. apply H.
+  eapply IF_apply. apply H.
+  intro. subst. apply H0. reflexivity.
+Qed.
+
+Reserved Notation " t '~' t' " (at level 40).
+Inductive path_equiv: relation trace__S :=
+| pe_refl: forall t, t ~ t
+| pe_sym: forall t t', t ~ t' -> t' ~ t
+| pe_trans: forall t1 t2 t3, t1 ~ t2 -> t2 ~ t3 -> t1 ~ t3
+| pe_interference_free: forall t t' e1 e2,
+    interference_free e1 e2 ->
+    ((((t :: e1) :: e2)) ++ t') ~ ((((t :: e2) :: e1)) ++ t')
+  where " t '~' t' " := (path_equiv t t').
+
+Global Instance refl_path_eq: Reflexive path_equiv.
+Proof. intro. apply pe_refl. Qed.
+
+Global Instance sym_path_eq: Symmetric path_equiv.
+Proof. intro. apply pe_sym. Qed.
+
+Global Instance trans_path_eq: Transitive path_equiv.
+Proof. intro. apply pe_trans. Qed.
+
+Lemma path_equiv_extend: forall t t' a,
+    t ~ t' -> (t :: a) ~ (t' :: a).
+Proof.
+  intros. induction H.
+  - reflexivity.
+  - symmetry. assumption.
+  - transitivity (t2::a); assumption.
+  - rewrite app_comm_cons. apply pe_interference_free. assumption.
+Qed.
+
+Theorem equiv_acc_subst: forall t t', t ~ t' -> acc_subst id_sub t = acc_subst id_sub t'.
+Proof.
+  intros. induction H; try auto. rewrite IHpath_equiv1. assumption.
+  (* the interesting case*)
+  induction t'.
+  - destruct e1, e2; simpl; try reflexivity.
+    apply IF_simultaneous_subst. assumption.
+  - destruct a; simpl.
+    + rewrite IHt'. reflexivity.
+    + assumption.
+Qed.
+
+Theorem diamond_property: forall s1 s2 s1' s2' t e1 e2,
+    red__S (t, <{s1 || s2}>) (t :: e1, <{s1' || s2}>) ->
+    red__S (t, <{s1 || s2}>) (t :: e2, <{s1 || s2'}>) ->
+    red__S (t :: e1, <{s1' || s2}>) ((t :: e1) :: e2, <{s1' || s2'}>) /\
+    red__S (t :: e2, <{s1 || s2'}>) ((t :: e2) :: e1, <{s1' || s2'}>)
+.
+Proof.
+  split.
+  - dependent destruction H0. dependent destruction H1;
+      inversion x0; inversion x; subst.
+    + dependent destruction H0;
+        apply cons_neq' in x; contradiction.
+    + dependent destruction H0;
+        apply context_injective in H5; try discriminate; try assumption; symmetry in H5;
+        [ apply SIf_true_disjoint in H5
+        | apply SIf_false_disjoint in H5
+        | apply SSeq_disjoint in H5
+        | apply SPar_right_disjoint in H5
+        | apply SPar_left_disjoint in H5];
+        contradiction.
+    + dependent destruction H0;
+        try (apply cons_neq' in x; contradiction);
+        try (apply ctx_red_intro with (C := fun s => SPar s1' (C s));
+             [constructor | constructor; assumption]).
+  - dependent destruction H. dependent destruction H0;
+      inversion x0; inversion x; subst.
+    + dependent destruction H;
+        apply cons_neq' in x; contradiction.
+    + dependent destruction H;
+        try (apply cons_neq' in x; contradiction);
+        try (apply ctx_red_intro with (C := fun s => SPar (C s) s2');
+             [constructor | constructor; assumption]).
+    + dependent destruction H;
+        apply context_injective in H6; try assumption; apply symmetry in H6;
+        [ discriminate
+        | apply SIf_true_disjoint in H6
+        | apply SIf_false_disjoint in H6
+        | apply SSeq_disjoint in H6
+        | apply SPar_right_disjoint in H6
+        | apply SPar_left_disjoint in H6];
+        contradiction.
+Qed.
+
+Theorem POR_bisimulation: forall s t1 s' t1' t2,
+    t1 ~ t2 -> red__S (t1, s) (t1', s') ->
+    exists t2', red__S (t2, s) (t2', s') /\ t1' ~ t2'.
+Proof.
+  intros. inversion H0; subst. inversion H4; subst; eexists; split;
+    try (constructor; [constructor | assumption]);
+    try (apply path_equiv_extend);
+    assumption.
 Qed.
